disj/PathSplits.v
@@ -1,37 +1,132 @@
-Require Export LiftShift LoopSplits.
+Require Export LiftShift LoopSplits CncLoop.
+
+Lemma both_exit_or_teq `(C : redCFG) q1 q2 p j1 j2 i
+      (Hedge1 : (q1,j1) -t> (p,i))
+      (Hedge2 : (q2,j2) -t> (p,i))
+  : exists h, exit_edge h q1 p /\ exit_edge h q2 p \/ j1 = j2 /\ deq_loop p q1.
+Proof.
+Admitted.
+
+Lemma edge_edge_loop `(C : redCFG) q1 q2 p
+      (Hedge1 : edge__P q1 p)
+      (Hedge2 : edge__P q2 p)
+  : eq_loop q1 q2.
+Proof.
+Admitted.
 
 Section disj.
 
   Context `(C : redCFG).
-(*  Variable (t1 t2 : list (Lab * Tag)) (r1 r2 : list (Lab * Tag)) (q1 q2 s : Lab) (j1 j2 k : Tag).
-  Hypotheses (Hlc : last_common' t1 t2 r1 r2 (s,k))
-             (Hpath1 : TPath (root,start_tag) (q1,j1) t1)
-             (Hpath2 : TPath (root,start_tag) (q2,j2) t2).*)
-(*             (Hloop : eq_loop q1 q2)
-             (Htag : tl j1 = tl j2)
-             (Htagleq : hd 0 j1 <= hd 0 j2). *)
-  (*
+  Variables (q1 q2 s p qs1 qs2 : Lab)
+            (i j k js1 js2 : Tag)
+            (t1 t2 r1 r2 : list (@Coord Lab)).
+  
+  Variable (D : disjPaths C q1 q2 s t1 t2 r1 r2 j j k i i p p qs1 qs2 js1 js2).
 
-  Hypotheses (Htag : tl j1 = tl j2)
-             (Htagleq : hd 0 j1 <= hd 0 j2)
-             (Hextra : j1 = j2 -> exists π, CPath q2 h (π :r: q2) /\ Disjoint (map fst r1) π).*) 
+  Lemma lc_join_split_base'
+        (Heq : eq_loop q1 s)
+    : (s,qs1,qs2) ∈ path_splits p.
+  Admitted.
+  
+  Lemma lc_join_split_base
+        (Heq : eq_loop q1 s)
+    : (s,qs1,qs2) ∈ splits p.
+  Proof.
+    eapply splits_spec.
+    left. eapply lc_join_split_base';auto.
+  Qed.
 
-  Lemma both_exit_or_teq q1 q2 p j1 j2 i
-        (Hedge1 : (q1,j1) -t> (p,i))
-        (Hedge2 : (q2,j2) -t> (p,i))
-    : exists h, exit_edge h q1 p /\ exit_edge h q2 p \/ j1 = j2.
+End disj.
+Section disj.
+
+  Context `(C : redCFG).
+  Variables (q1 q2 s p qs1 qs2 : Lab)
+            (i j k js1 js2 : Tag)
+            (t1 t2 r1 r2 : list (@Coord Lab)).
+  
+  Hypotheses (D : disjPaths C q1 q2 s t1 t2 r1 r2 j j k i i p p qs1 qs2 js1 js2)
+             (Hpqdeq : deq_loop p q1).
+
+  Lemma ps_non_contains
+    : ~ loop_contains p s.
   Proof.
   Admitted.
 
-  Variables (p q1 q2 s : Lab) (i j k : Tag) (t1 t2 r1 r2 : list (@Coord Lab)). 
-  Hypotheses (Hlc : last_common' ((q1, j) :: t1) ((q2, j) :: t2) r1 r2 (s, k))
-             (Hneq : q1 <> q2)
-             (Hpath1 : TPath (root, start_tag) (p, i) ((p, i) :: (q1, j) :: t1))
-             (Hpath2 : TPath (root, start_tag) (p, i) ((p, i) :: (q2, j) :: t2)).
+  Lemma sep_pq_eq_p
+    : forall h, loop_contains h p -> ~ loop_contains h q1 -> h = p.
+  Admitted.
 
-  Lemma psplits_q1_eq_q2
-    : eq_loop q1 q2.
+  Lemma ocnc_loop_pq s'
+        (Hocnc : ocnc_loop s p s')
+    : ocnc_loop s q1 s'.
   Proof.
+  Admitted.
+
+  Lemma deq_ps_deq_qs
+        (Hdeq : deq_loop p s)
+    : deq_loop q1 s.
+  Proof.
+    (* case destinction on the edge q->p:
+     * if exit contradition bc. tags
+     * if normal or back_edge then eq_loop
+     * if entry then show that there must be an outer backedge to re-enter p 
+     * which is a contradiction to the non-existence of outer backedges on disjoint paths
+     *)
+  Admitted.
+
+  Theorem lc_join_split'
+    : (s,qs1,qs2) ∈ splits p.
+  Proof.
+    assert (deq_loop s q1) as Hsdeq.
+    { eapply s_deq_q;destruct D;eauto. }
+    decide (deq_loop p s).
+    - eapply deq_ps_deq_qs in d. eapply lc_join_split_base. eauto. split;eauto.
+    - rename n into Hndeq.
+      specialize (ex_impl_dP D Hndeq Hpqdeq) as I. destructH.
+      specialize (lift_disjPaths (I:=I)) as Q.
+      assert (e1' = e2') as Eeq.
+      { eapply subtype_extensionality.
+        rewrite <-He1. rewrite <-He2. reflexivity. }
+      subst e2'.
+      assert (eq_loop (C:=local_impl_CFG C p) q1' s') as Hqseq.
+      { specialize (ocnc_loop_pq Hocnc) as Hq.
+        split.
+        - eapply ocnc_loop_exit in Hq. admit. (* bc. dep q1' = dep q1 & dep e = dep s' *)
+        - unfold ocnc_loop,cnc_loop in Hq. admit.
+      }
+      eapply lc_join_split_base in Q as Hsplit. 2:auto.
+      setoid_rewrite splits_spec.
+      right. right.
+      exists (`s'),(`qs1'),(`qs2').
+      split.
+      + specialize (@splits_path_splits__imp _ _ _ _ C p e1' s' qs1' qs2') as QQ.
+        exploit QQ.
+        * rewrite He1. reflexivity.
+        * eapply lc_join_split_base';eauto.
+        * destruct I. setoid_rewrite <-He1 in QQ. apply QQ. 
+      + specialize (Nat.lt_trichotomy n1 n2) as [Nlt|[Neq|Nlt]];[left| |right].
+        * eapply lc_disj_exits_lsplits'.
+          -- eapply disjPathsE_shift_lt.
+          -- cbn. reflexivity.
+          -- cbn. clear - Nlt; omega.
+          -- intro N. exfalso. inversion N. rewrite H0 in Nlt. clear - Nlt. omega.
+        * specialize (disjPathsE_shift_eq Neq) as Dshift.
+          eapply disj_latch_path_or in Dshift as Hπ. 2: clear - Neq;f_equal;eauto.
+          destruct Hπ as [π [Hπ | Hπ]];[left|right].
+          -- eapply lc_disj_exits_lsplits'. 1:eapply Dshift. 1,2:cbn;eauto.
+             1:rewrite Neq;reflexivity.
+             intro N. eexists;eauto.
+          -- eapply splits'_sym.
+             eapply lc_disj_exits_lsplits'. 1:eapply disjPathsE_sym;eapply Dshift. 1,2:cbn;eauto.
+             1: rewrite Neq;reflexivity.
+             intro N. eexists;eauto. 
+        * eapply splits'_sym.
+          eapply lc_disj_exits_lsplits'.
+          -- eapply disjPathsE_sym. 
+             eapply disjPathsE_shift_lt2.
+          -- cbn. reflexivity.
+          -- cbn. clear - Nlt; omega.
+          -- intro N. exfalso. inversion N. rewrite H0 in Nlt. clear - Nlt. omega.
   Admitted.
     
 End disj.
@@ -44,24 +139,25 @@ Theorem lc_join_split `{C : redCFG} t1 t2 (p q1 q2 s : Lab) (i j1 j2 k : Tag)
         (Hpath2 : TPath (root,start_tag) (p,i) ((p,i) :: (q2,j2) :: t2))
   : exists qq qq', (s,qq,qq') ∈ splits p.
 Proof.
+  inversion Hpath1. inversion Hpath2. subst.
+  rename H0 into Hpath1'. rename H5 into Hpath2'.
+  rename H3 into Hedge1. rename H8 into Hedge2.
+  replace b with (q1,j1) in *. clear b.
+  2: { eapply path_front in Hpath1'. auto. }
+  replace b0 with (q2,j2) in *. clear b0.
+  2: { eapply path_front in Hpath2'. auto. }
   specialize (both_exit_or_teq (C:=C)) as Hbet. specialize (Hbet q1 q2 p j1 j2 i).
   exploit Hbet.
-  1: inversion Hpath1;subst;path_simpl' H0;eauto.
-  1: inversion Hpath2;subst;path_simpl' H0;eauto.
   destructH.
   destruct Hbet.
   - destructH. eapply lc_disj_exit_lsplits in Hlc;eauto.
     destructH. do 2 eexists. eapply splits_spec. right. left. eexists. eauto.
-  - subst j2. rewrite last_common'_iff in Hlc. destruct Hlc as [r1 [r2 Hlc]].
-    inversion Hpath1. inversion Hpath2. subst.
-    rename H0 into Hpath1'. rename H5 into Hpath2'.
-    rename H3 into Hedge1. rename H8 into Hedge2.
-    replace b with (q1,j1) in *. clear b.
-    2: { eapply path_front in Hpath1'. auto. }
-    replace b0 with (q2,j1) in *. clear b0.
-    2: { eapply path_front in Hpath2'. auto. } 
-    decide (deq_loop q1 s).
-    + eapply s_deq_q in Hlc;eauto. 2: eapply psplits_q1_eq_q2;eauto. admit.
+  - destruct H. subst j2.
+    rewrite last_common'_iff in Hlc. destructH.
+    eexists;eexists.
+    eapply lc_join_split'. 2:eauto.
+    econstructor;eauto.
+    + rewrite <-surjective_pairing. eapply succ_cons. admit.
     + admit.
-  
+    + eapply edge_edge_loop; unfold tcfg_edge,tcfg_edge' in *; do 2 destructH; eauto.
 Admitted.
